prove lenient_wp_seq

theories/iris/language/lenient_wp.v
@@ -1,30 +1,159 @@
-From RWasm.iris.language Require Import iris_wp_def.
+From RWasm.iris.rules Require Import iris_rules_structural iris_rules_trap.
+From RWasm.iris.language Require Import iris_wp_def logpred.
+Import iris.algebra.list.
+From iris.proofmode Require Import base tactics classes.
+Set Bullet Behavior "Strict Subproofs".
+
 Section lenient_wp.
   Context `{!wasmG Σ}.
-  Print iris.val.
   Open Scope bi_scope.
 
-  Record logpred :=
-    MkLP {
-        lp_val: list value → iProp Σ;
-        lp_trap: iPropI Σ;
-        lp_br: ∀ n: nat, valid_holed n → iProp Σ;
-        lp_ret: simple_valid_holed → iProp Σ;
-        lp_host: function_type → hostfuncidx → list value → llholed → iProp Σ;
-      }.
+  Section wp_params.
+  Variables (s: stuckness) (E: coPset).
 
-  Definition denote_logpred (Φ: logpred) : val -> iProp Σ :=
-    λ w, match w with
-         | immV vs => Φ.(lp_val) vs
-         | trapV => ↪[BAIL] ∗ Φ.(lp_trap)
-         | brV i lh => Φ.(lp_br) i lh
-         | retV lh => Φ.(lp_ret) lh
-         | callHostV ft hidx vs lh => Φ.(lp_host) ft hidx vs lh
-         end.
+  Definition lp_notrap (Φ: logpred) : val -> iProp Σ := 
+    λ lv,
+      match lv with
+      | trapV => False
+      | _ => lp_noframe Φ lv
+      end.
 
-  Notation "⟦ Φ ⟧" := (denote_logpred Φ).
+  Definition lenient_wp (es: expr) (Φ: logpred): iProp Σ :=
+    wp s E es (denote_logpred Φ).
 
-  Definition lenient_wp (s: stuckness) (E: coPset) (es: expr) (Φ: logpred): iProp Σ :=
-    wp s E es ⟦Φ⟧.
+  Definition lenient_wp_ctx (es: expr) (Φ: logpred) (i: nat) (lh: lholed) : iProp Σ :=
+    wp_wasm_ctx s E es (denote_logpred Φ) i lh.
+
+  Lemma lp_trap_sep (Φ Ψ: logpred) :
+    lp_trap (Φ ∗ Ψ) ⊣⊢ lp_trap Φ ∗ lp_trap Ψ.
+  Proof.
+    reflexivity.
+  Qed.
+
+  (* TODO move this to the structural rules file with wp_seq_can_trap_ctx and the rest of those lemmas *)
+  Lemma wp_seq_can_trap (Φ Ψ : iris.val -> iProp Σ) (es1 es2 : language.expr wasm_lang) (Φf : datatypes.frame -> iProp Σ) (Φt : iProp Σ) :
+    (Ψ trapV ={E}=∗ ⌜False⌝) ∗
+    (∀ f, ↪[frame] f ∗ Φt ∗ Φf f -∗ Φ trapV) ∗
+    WP es1 @ NotStuck; E {{ w, (⌜w = trapV⌝ ∗ Φt ∨ Ψ w) ∗ ∃ f0, ↪[frame] f0 ∗ Φf f0 }} ∗
+    (∀ w (f0: datatypes.frame),
+        Ψ w ∗ ↪[frame] f0 ∗ Φf f0 -∗
+        WP (of_val w ++ es2) @ s; E {{ v, Φ v }})
+    ⊢ WP (es1 ++ es2) @ s; E {{ v, Φ v }}.
+  Proof.
+    iIntros "(HΨnotrap & Hframetrap & Hes1 & Hes2)".
+    iApply wp_wasm_empty_ctx.
+    iApply wp_seq_can_trap_ctx_precise; iFrame.
+    iIntros (w f0) "(Hw & Hf0 & HΦf)".
+    Locate "CTX_EMPTY".
+    Search (LH_base nil nil) wp_wasm_ctx.
+    unfold wp_wasm_ctx.
+    iIntros (LI Hfill).
+    assert (LI = (iris.of_val w ++ es2)).
+    {
+      cbn in *.
+      rewrite app_nil_r in Hfill.
+      by destruct (@seq.eqseqP _ LI (iris.of_val w ++ es2)).
+    }
+    subst LI.
+    iApply "Hes2".
+    iFrame.
+  Qed.
+
+  (*
+  Definition has_a_frame (Φ: iProp Σ) :=
+    ∃ Φ' (f: datatypes.frame), □(Φ ∗-∗ Φ' ∗ ↪[frame] f).
+
+  Lemma wp_seq_can_trap' (Φ Ψ : iris.val -> iProp Σ) (Ψt: iProp Σ) (es1 es2 : language.expr wasm_lang) f :
+    ↪[frame] f ∗
+    (∀ w, has_a_frame (Ψ w)) ∗
+    (∀ w, has_a_frame (Φ w)) ∗
+    (((Ψ trapV ={E}=∗ ⌜False⌝)) ∗
+     (Ψt -∗ Φ trapV) ∗
+     (WP es1 @ NotStuck; E {{ w, (⌜w = trapV⌝ ∗ Ψt) ∨ Ψ w}}) ∗
+     ∀ w, Ψ w -∗ WP (iris.of_val w ++ es2) @ s; E {{ v, Φ v }})%I
+     ⊢ WP (es1 ++ es2) @ s; E {{ v, Φ v }}.
+  Proof.
+    iLöb as "IH" forall (Φ Ψ Ψt es1 es2 f).
+    iIntros "(Hf & HfΨ & HfΦ & Hnotrap & Httrap & Hes1 & Hes2)".
+    repeat rewrite wp_unfold /wp_pre /=.
+    destruct (iris.to_val es1) as [vs|] eqn:Hes1tov.
+    {
+      iMod ("Hes1").
+      iDestruct "Hes1" as "[[-> Hes1] | Hes1]".
+      {
+        apply to_val_trap_is_singleton in Hes1tov as ->.
+        destruct es2; cycle 1.
+        {
+          iSpecialize ("Httrap" with "Hes1").
+          iAssert (has_a_frame (Φ trapV)) with "[HfΦ]" as "HfΦ'".
+          iApply "HfΦ".
+          iDestruct "HfΦ'" as (Φ' fr) "#Hsplit".
+          iAssert (Φ' ∗ ↪[frame] fr) with "[Httrap]" as "[HΦ' Hfr]".
+          by iApply "Hsplit".
+          iApply (wp_wand _ _ _ (λ v, Φ' ∗ ↪[frame] fr) with "[HΦ' Hfr]").
+          change [AI_trap] with ([] ++ [AI_trap]).
+          rewrite -app_assoc.
+          iApply (wp_trap with "[HΦ'] [$Hfr]").
+          done.
+          iFrame.
+          done.
+          iApply "Hsplit" in "Httrap".
+
+
+          iApply "Hes2".
+          assert (iris.to_val ([AI_trap] ++ a :: es2) = None) as Hnone
+              by (rewrite -(app_nil_l [AI_trap]) -app_assoc; apply to_val_not_trap_interweave; auto).
+          rewrite /has_a_frame.
+          iRewrite "HfΦ".
+          Search wp AI_trap.
+          eapply wp_trap.
+          rewrite Hnone.
+          congruence.
+
+        }
+          eapply to_val_None_lfilled in Hnone; [|eauto].
+        
+      unfold iris
+      iDestruct H
+
+      eapply lfilled_to_val_app in Hes1tov as HH;eauto.
+      destruct HH as [vs' [Hvs' Hfilled']].
+      unfold iris_wp_def.to_val in Hvs'.
+    rewrite Hvs'.
+      apply to_val_trap_is_singleton in Hvs'.
+      *)
+
+  End wp_params.
+
+  Lemma lenient_wp_seq s E (Φ Ψ: logpred) es1 es2 :
+    lenient_wp NotStuck E es1 Ψ ∗
+    (* trap case: old frame and trap conditions imply the new ones *)
+    (∀ f, lp_trap Ψ ∗ lp_fr Ψ f -∗ lp_trap Φ ∗ lp_fr Φ f) ∗
+    (* non-trap case: old frame and non-trap conditions imply the new wp *)
+    (∀ w f, lp_notrap Ψ w ∗ ↪[frame] f ∗ lp_fr Ψ f -∗ lenient_wp s E (of_val w ++ es2) Φ)
+    ⊢ lenient_wp s E (es1 ++ es2) (Φ).
+  Proof.
+    iIntros "(Hes1 & Htrapimpl & Hes2)".
+    iApply (wp_seq_can_trap s E _ (lp_notrap Ψ) _ _ Ψ.(lp_fr) (↪[BAIL] ∗ Ψ.(lp_trap))).
+    iSplitR; [done |].
+    unfold lenient_wp.
+    iSplitL "Htrapimpl".
+    {
+      iIntros (f0) "[Hf0 [[Hbail Htrap] Hfr]]".
+      iFrame.
+      iApply "Htrapimpl".
+      iFrame.
+    }
+    iSplitR "Hes2".
+    - iApply (wp_wand with "[Hes1]").
+      + iApply "Hes1".
+      + iIntros (v). destruct v; unfold denote_logpred; cbn; iIntros "[Hlog Hfr]";
+          try iFrame.
+        iLeft.
+        by iFrame.
+    - iIntros (w f) "(Hnotrap & Hfr & Hfrcond)".
+      iApply "Hes2".
+      iFrame.
+  Qed.
 
 End lenient_wp.
